src/sequential/SeqLiftAux.v
@@ -1,0 +1,186 @@
+Require Import RelationClasses.
+
+From sflib Require Import sflib.
+From Paco Require Import paco.
+
+From PromisingLib Require Import Axioms.
+From PromisingLib Require Import Basic.
+From PromisingLib Require Import Loc.
+From PromisingLib Require Import DenseOrder.
+From PromisingLib Require Import Language.
+
+Require Import Event.
+Require Import Time.
+Require Import View.
+Require Import Cell.
+Require Import Memory.
+Require Import MemoryFacts.
+Require Import TView.
+Require Import Local.
+Require Import Thread.
+Require Import Configuration.
+
+Require Import Cover.
+Require Import MemorySplit.
+Require Import MemoryMerge.
+Require Import FulfillStep.
+Require Import MemoryProps.
+
+Require Import gSimAux.
+Require Import LowerMemory.
+Require Import JoinedView.
+
+Require Import MaxView.
+Require Import Delayed.
+
+Require Import Lia.
+
+Require Import JoinedView.
+Require Import SeqLift.
+Require Import gSimulation.
+Require Import Simple.
+
+Require Import Pred.
+
+Require Import SeqLiftStep.
+
+
+Lemma sim_thread_deflag_match_aux2
+      f0 vers flag_src flag_tgt vs_src vs_tgt
+      mem_src0 mem_tgt lc_src0 lc_tgt sc_src sc_tgt
+      loc
+      (SIM: sim_thread
+              f0 vers flag_src flag_tgt vs_src vs_tgt
+              mem_src0 mem_tgt lc_src0 lc_tgt sc_src sc_tgt)
+      (CONSISTENT: Local.promise_consistent lc_tgt)
+      (LOCALSRC: Local.wf lc_src0 mem_src0)
+      (LOCALTGT: Local.wf lc_tgt mem_tgt)
+      (MEMSRC: Memory.closed mem_src0)
+      (MEMTGT: Memory.closed mem_tgt)
+      (SCSRC: Memory.closed_timemap sc_src mem_src0)
+      (SCTGT: Memory.closed_timemap sc_tgt mem_tgt)
+      (WF: Mapping.wfs f0)
+      (FLAG: flag_src loc = true)
+      (VAL: option_rel Const.le (vs_tgt loc) (vs_src loc))
+      lang st
+  :
+    exists lc_src1 mem_src1 f1,
+      (<<STEPS: rtc (tau (@pred_step is_promise _))
+                    (Thread.mk lang st lc_src0 sc_src mem_src0)
+                    (Thread.mk _ st lc_src1 sc_src mem_src1)>>) /\
+      (<<SIM: sim_thread
+                f1 vers
+                (fun loc0 => if Loc.eq_dec loc0 loc then false else flag_src loc0)
+                (fun loc0 => if Loc.eq_dec loc0 loc then false else flag_tgt loc0)
+                vs_src vs_tgt
+                mem_src1 mem_tgt lc_src1 lc_tgt sc_src sc_tgt>>) /\
+      (<<WF: Mapping.wfs f1>>) /\
+      (<<MAPLE: Mapping.les f0 f1>>) /\
+      (<<UNCH: forall loc0 (NEQ: loc0 <> loc), f1 loc0 = f0 loc0>>) /\
+      (<<MAPFUTURE: map_future_memory f0 f1 mem_src1>>)
+.
+Proof.
+  inv SIM. hexploit (MAXSRC loc). intros MAXTSSRC.
+  hexploit (MAXTGT loc). intros MAXTSTGT.
+  destruct (vs_src loc) eqn:VSRC; cycle 1.
+  { hexploit max_value_src_flag_none; eauto. i. clarify. }
+  inv MAXTSSRC. hexploit MAX; eauto. i. des.
+  destruct (vs_tgt loc) eqn:VTGT; ss.
+  inv MAXTSTGT. hexploit MAX1; eauto. i. des.
+  assert (TS: srctm loc = View.rlx (TView.cur tvw) loc).
+  { inv LOCAL. auto. }
+  hexploit sim_memory_top; eauto. intros TOP.
+  hexploit (@shifted_mapping_exists (f0 loc) (srctm loc)); eauto. i. des.
+Admitted.
+
+
+
+(*   { rewrite TOP in TOP. *)
+
+(*   i. des. rewrite *)
+
+
+
+(* Lemma add_promises_latest lang (st: lang.(Language.state)) tvw sc loc msgs: *)
+(*   forall prom0 mem0 *)
+(*          (WFMSGS: wf_cell_msgs msgs) *)
+(*          (MLE: Memory.le prom0 mem0) *)
+(*          (MEM: Memory.closed mem0) *)
+(*          (FORALL: List.Forall *)
+(*                     (fun '(from, to, msg) => (__guard__((<<MAX: Time.le (Memory.max_ts loc mem0) from>>) \/ (<<RESERVE: msg = Message.reserve>>) /\ (<<DISJOINT: forall to2 from2 msg2 (GET: Memory.get loc to2 mem0 = Some (from2, msg2)), Interval.disjoint (from, to) (from2, to2)>>))) /\ (<<TS: Time.lt from to>>) /\ (<<MSGTO: Memory.message_to msg loc to>>) /\ (<<WF: Message.wf msg>>) /\ (<<CLOSED: semi_closed_message msg mem0 loc to>>)) msgs), *)
+
+
+(*   { *)
+
+(* ; eauto. *)
+(*   hexploit (MAXSRC loc). *)
+
+
+(*     { speeapply MAXSRC. *)
+
+(*   2:{ *)
+
+(* hexploit NONMAX; eauto. i. des. *)
+
+
+
+(* sim_memory *)
+(*   inv SIM. *)
+(*   hexploit sim_memory_top; eauto. intros TOP. *)
+
+
+(* Lemma shifted_mapping_exists (f0: Mapping.t) *)
+(*       (ts: Time.t) (fts: Time.t) *)
+(*       (TOP: top_time fts f0) *)
+(*       (WF: Mapping.wf f0) *)
+(*   : *)
+(*     exists f1, *)
+(*       (<<SAME: forall to fto *)
+(*                       (TS: Time.lt to ts) *)
+(*                       (MAP: sim_timestamp_exact f0 f0.(Mapping.ver) fto to), *)
+(*           sim_timestamp_exact f1 f1.(Mapping.ver) fto to>>) /\ *)
+(*       (<<TS: sim_timestamp_exact f1 f1.(Mapping.ver) fts ts>>) /\ *)
+(*       (<<LE: Mapping.le f0 f1>>) /\ *)
+(*       (<<WF: Mapping.wf f1>>) /\ *)
+(*       (<<CLOSED: forall ts, Mapping.closed f1 f1.(Mapping.ver) ts <-> Mapping.closed f0 f0.(Mapping.ver) ts>>) *)
+(* . *)
+
+
+
+(* Admitted. *)
+
+(* Lemma sim_thread_deflag_unmatch_aux2 *)
+(*       f0 vers flag_src flag_tgt vs_src vs_tgt *)
+(*       mem_src0 mem_tgt lc_src0 lc_tgt sc_src sc_tgt *)
+(*       loc ts *)
+(*       (SIM: sim_thread *)
+(*               f0 vers flag_src flag_tgt vs_src vs_tgt *)
+(*               mem_src0 mem_tgt lc_src0 lc_tgt sc_src sc_tgt) *)
+(*       (CONSISTENT: Local.promise_consistent lc_tgt) *)
+(*       (LOCALSRC: Local.wf lc_src0 mem_src0) *)
+(*       (LOCALTGT: Local.wf lc_tgt mem_tgt) *)
+(*       (MEMSRC: Memory.closed mem_src0) *)
+(*       (MEMTGT: Memory.closed mem_tgt) *)
+(*       (SCSRC: Memory.closed_timemap sc_src mem_src0) *)
+(*       (SCTGT: Memory.closed_timemap sc_tgt mem_tgt) *)
+(*       (WF: Mapping.wfs f0) *)
+(*       (FLAG: flag_src loc = Some ts) *)
+(*       lang st *)
+(*   : *)
+(*     exists lc_src1 mem_src1 f1 flag, *)
+(*       (<<STEPS: rtc (tau (@pred_step is_promise _)) *)
+(*                     (Thread.mk lang st lc_src0 sc_src mem_src0) *)
+(*                     (Thread.mk _ st lc_src1 sc_src mem_src1)>>) /\ *)
+(*       (<<SIM: sim_thread *)
+(*                 f1 vers *)
+(*                 (fun loc0 => if Loc.eq_dec loc0 loc then None else flag_src loc0) *)
+(*                 (fun loc0 => if Loc.eq_dec loc0 loc then flag else flag_tgt loc0) *)
+(*                 vs_src vs_tgt *)
+(*                 mem_src1 mem_tgt lc_src1 lc_tgt sc_src sc_tgt>>) /\ *)
+(*       (<<WF: Mapping.wfs f1>>) /\ *)
+(*       (<<MAPLE: Mapping.les f0 f1>>) /\ *)
+(*       (<<UNCH: forall loc0 (NEQ: loc0 <> loc), f1 loc0 = f0 loc0>>) /\ *)
+(*       (<<MAPFUTURE: map_future_memory f0 f1 mem_src1>>) *)
+(* . *)
+(* Proof. *)
+(* Admitted. *)
