src/sequential/SeqLiftInterference.v
@@ -44,7 +44,7 @@ Require Import Simple.
 Require Import Pred.
 
 Require Import SeqLiftStep.
-
+Require Import FutureCertify.
 
 Lemma wf_release_vers_versions_le
       vers0 vers1 prom rel_vers
@@ -57,37 +57,87 @@ Proof.
   esplits; eauto.
 Qed.
 
-Lemma undef_added_failure lang st lc sc0 mem0 sc1 mem1
-      (CONSISTENT: Thread.consistent (Thread.mk lang st lc sc0 mem0))
-      (MEMLE: Memory.future_weak mem0 mem1)
-      (SCLE: TimeMap.le sc0 sc1)
-      (LOCAL: Local.wf lc mem0)
-      (MEM0: Memory.closed mem0)
-      (SC0: Memory.closed_timemap sc0 mem0)
-      (MEM1: Memory.closed mem1)
-      (SC1: Memory.closed_timemap sc1 mem1)
-      loc from0 to0 msg from1 to1
-      (GET0: Memory.get loc to0 lc.(Local.promises) = Some (from0, msg))
-      (MSG: msg <> Message.reserve)
-      (GET1: Memory.get loc to1 mem1 = Some (from1, Message.undef))
-      (TS: Time.lt to0 to1)
-      (NONE: Memory.get loc to1 lc.(Local.promises) = None)
+Lemma max_value_no_flag_le f vers srctm flag_src flag_tgt lc_src lc_tgt mem_src mem_tgt loc v_src v_tgt
+      (MEM: sim_memory srctm flag_src f vers mem_src mem_tgt)
+      (LOCAL: sim_local f vers srctm flag_src flag_tgt lc_src lc_tgt)
+      (FLAGSRC: flag_src loc = false)
+      (FLAGTGT: flag_tgt loc = false)
+      (MAXSRC: max_value_src loc (Some v_src) mem_src lc_src)
+      (MAXTGT: max_value_tgt loc (Some v_tgt) mem_tgt lc_tgt)
+      (LOCALWF: Local.wf lc_tgt mem_tgt)
+      (CONSISTENT: Local.promise_consistent lc_tgt)
+      (WF: Mapping.wfs f)
   :
-  Thread.steps_failure (Thread.mk _ st lc sc1 mem1).
+    Const.le v_tgt v_src.
 Proof.
-Admitted.
+  hexploit no_flag_max_value_same; eauto.
+  i. des. inv MAX. inv MAXTGT.
+  hexploit MAX0; eauto. i. des. hexploit MAX; eauto. i. des.
+  eapply max_readable_inj in MAX1; eauto. des. subst. auto.
+Qed.
+
+Lemma max_value_sim_timestamp_exact
+      f vers srctm flag_src flag_tgt lc_src lc_tgt mem_src mem_tgt loc v_src v_tgt
+      (MEM: sim_memory srctm flag_src f vers mem_src mem_tgt)
+      (LOCAL: sim_local f vers srctm flag_src flag_tgt lc_src lc_tgt)
+      (FLAGSRC: flag_src loc = false)
+      (FLAGTGT: flag_tgt loc = false)
+      (MAXSRC: max_value_src loc (Some v_src) mem_src lc_src)
+      (MAXTGT: max_value_tgt loc (Some v_tgt) mem_tgt lc_tgt)
+      (LOCALWF: Local.wf lc_tgt mem_tgt)
+      (CONSISTENT: Local.promise_consistent lc_tgt)
+      (WF: Mapping.wfs f)
+  :
+    sim_timestamp_exact
+      (f loc) ((f loc).(Mapping.ver))
+      (lc_src.(Local.tview).(TView.cur).(View.pln) loc)
+      (lc_tgt.(Local.tview).(TView.cur).(View.pln) loc).
+Proof.
+  inv MAXTGT. hexploit MAX; eauto. i. des. inv MAX0.
+  hexploit sim_memory_get; eauto; ss. i. des.
+  assert (to_src = (lc_src.(Local.tview).(TView.cur).(View.pln) loc)); [|clarify].
+  inv LOCAL. ss. eapply TimeFacts.antisym.
+  { destruct (Time.le_lt_dec to_src (View.pln (TView.cur tvw_src) loc)); ss.
+    exfalso. inv MAXSRC. hexploit MAX0; eauto. i. des. inv MAX2.
+    hexploit MAX3; eauto.
+    { inv MSG; ss. }
+    i. hexploit sim_promises_get_if; eauto. i. des; clarify.
+    hexploit sim_timestamp_exact_unique.
+    { eapply TO0. }
+    { eapply TO. }
+    { eauto. }
+    { eapply mapping_latest_wf_loc. }
+    i. subst. exploit CONSISTENT; eauto.
+    { inv MSG; inv MSG0; ss. }
+    i. ss. eapply Time.lt_strorder. eapply TimeFacts.lt_le_lt.
+    { eapply x. }
+    { eapply LOCALWF. }
+  }
+  { eapply sim_timestamp_le.
+    { eapply TVIEW; auto. }
+    { eauto. }
+    { refl. }
+    { eauto. }
+    { eapply mapping_latest_wf_loc. }
+  }
+Qed.
 
 Lemma sim_thread_future
+      loc_na
       f0 vers0 flag_tgt vs_src0 vs_tgt0
       mem_src0 mem_tgt0 lc_src0 lc_tgt0 sc_src0 sc_tgt0
 
       f1 vers1 mem_src1 mem_tgt1 sc_src1 sc_tgt1
+      lang st
       (SIM: sim_thread
               f0 vers0 (fun _ => false) flag_tgt vs_src0 vs_tgt0
               mem_src0 mem_tgt0 lc_src0 lc_tgt0 sc_src0 sc_tgt0)
 
       (MEMLESRC: Memory.future_weak mem_src0 mem_src1)
       (MEMLETGT: Memory.future_weak mem_tgt0 mem_tgt1)
+      (CLOSEDFUTURE: closed_future_tview loc_na lc_tgt0.(Local.tview) mem_tgt0 mem_tgt1)
+      (MAPFUTURE: map_future_memory f0 f1 mem_src1)
+
       (SCLESRC: TimeMap.le sc_src0 sc_src1)
       (SCLETGT: TimeMap.le sc_tgt0 sc_tgt1)
       (SIMMEM: sim_memory_interference f1 vers1 mem_src1 mem_tgt1)
@@ -107,14 +157,15 @@ Lemma sim_thread_future
       (SCTGT0: Memory.closed_timemap sc_tgt0 mem_tgt0)
       (WF0: Mapping.wfs f0)
       (VERS0: versions_wf f0 vers0)
-
       (MEMSRC1: Memory.closed mem_src1)
       (MEMTGT1: Memory.closed mem_tgt1)
       (SCSRC1: Memory.closed_timemap sc_src1 mem_src1)
       (SCTGT1: Memory.closed_timemap sc_tgt1 mem_tgt1)
       (WF1: Mapping.wfs f1)
       (VERS1: versions_wf f1 vers1)
-      lang st
+
+      (CONSISTENTPAST: Thread.consistent (Thread.mk lang st lc_src0 sc_src0 mem_src0))
+      (ATFLAG: forall loc (AT: ~ loc_na loc), flag_tgt loc = false)
   :
   exists lc_src2 sc_src2 mem_src2,
     (<<STEPS: rtc (@Thread.tau_step lang) (Thread.mk lang st lc_src0 sc_src1 mem_src1) (Thread.mk lang st lc_src2 sc_src2 mem_src2)>>) /\
@@ -127,38 +178,103 @@ Lemma sim_thread_future
                exists val_old,
                  (<<VS: vs_src0 loc = Some val_old>>) /\
                    (<<VAL: Const.le val_old val>>)>>) /\
-             (<<VALTGT: forall loc val (VAL: vs_tgt1 loc = Some val), vs_tgt0 loc = Some val>>) /\
-             (<<CLOSED: sim_closed_memory f1 mem_src2>>))
+             (<<VALTGT: forall loc val (VAL: vs_tgt1 loc = Some val) (NA: loc_na loc), vs_tgt0 loc = Some val>>))
 .
 Proof.
+  destruct (classic (exists loc from0 to0 msg from1 to1,
+                        (<<GET0: Memory.get loc to0 lc_src0.(Local.promises) = Some (from0, msg)>>) /\
+                        (<<MSG: msg <> Message.reserve>>) /\
+                        (<<GET1: Memory.get loc to1 mem_src1 = Some (from1, Message.undef)>>) /\
+                        (<<TS: Time.lt to0 to1>>) /\
+                        (<<NONE: Memory.get loc to1 mem_src0 = None>>))) as [|UNDEF].
+  { des. hexploit FutureCertify.undef_added_failure; eauto. i. esplits; eauto. }
+  assert (MEM1: sim_memory lc_src0.(Local.tview).(TView.cur).(View.rlx) (fun _ => false) f1 vers1 mem_src1 mem_tgt1).
+  { eapply sim_memory_interference_sim_memory; eauto. }
+  esplits; [refl|]. right.
+  hexploit (@max_values_src_exists mem_src1 lc_src0).
+  intros [vs_src1 MAXSRC1]. des.
+  inv SIM. inv LOCAL.
+  assert (VALSRC: forall loc val (VAL: vs_src1 loc = Some val),
+             exists val_old,
+               (<<VS: vs_src0 loc = Some val_old>>) /\
+               (<<VAL: Const.le val_old val>>)).
+  { i. specialize (MAXSRC loc). specialize (MAXSRC1 loc). inv MAXSRC. inv MAXSRC1.
+    hexploit MAX0; eauto. i. des. destruct (vs_src0 loc) eqn:EQ.
+    { hexploit MAX; eauto. i. des. inv MAX1. inv MAX2.
+      eapply Memory.future_weak_get1 in GET0; eauto; ss.
+      des. clarify. inv MSG_LE. esplits; eauto.
+    }
+    { exfalso. hexploit non_max_readable_future; eauto. }
+  }
+  hexploit (choice (fun loc v_tgt =>
+                      (<<MAX: max_value_tgt loc v_tgt mem_tgt1 (Local.mk tvw_tgt prom_tgt)>>) /\
+                      (<<OPTREL: option_rel (fun _ _ => True) (vs_src1 loc) v_tgt>>) /\
+                      (<<VALTGT: forall val (VAL: v_tgt = Some val) (NA: loc_na loc), vs_tgt0 loc = Some val>>))).
+  { intros loc. destruct (vs_src1 loc) eqn:VSRC.
+    2:{ exists None. splits; ss. }
+    hexploit VALSRC; eauto. i. des.
+    specialize (MAXSRC loc). inv MAXSRC. hexploit MAX; eauto. i. des. inv MAX0.
+    specialize (PERM loc). rewrite VS in PERM.
+    destruct (vs_tgt0 loc) eqn:VTGT0; ss.
+    specialize (MAXTGT loc). inv MAXTGT. hexploit MAX0; eauto. i. des. inv MAX2.
+    specialize (MAXSRC1 loc). inv MAXSRC1. hexploit MAX2; eauto. i. des. inv MAX4.
+    hexploit Memory.future_weak_get1.
+    { eapply MEMLETGT. }
+    { eauto. }
+    { ss. }
+    i. des. inv MSG_LE. exists (Some val). splits; auto.
+    { econs. i. inv VAL1. esplits. econs.
+      { eauto. }
+      { eauto. }
+      { i. hexploit sim_memory_get; ss.
+        { eapply MEM1. }
+        { eauto. }
+        { eauto. }
+        i. des. hexploit MAX5; eauto.
+        { eapply sim_timestamp_lt.
+          2:{ eauto. }
+          { eapply sim_timestamp_mon_ver.
+            { erewrite <- sim_timestamp_mon_mapping.
+              { eapply TVIEW; eauto. }
+              { eauto. }
+              { eapply mapping_latest_wf_loc. }
+              { eauto. }
+            }
+            { eapply MAPLE. }
+            { eauto. }
+            { eapply mapping_latest_wf_loc. }
+          }
+          { eauto. }
+          { eauto. }
+          { eapply mapping_latest_wf_loc. }
+        }
+        { inv MSG0; ss. }
+        i. hexploit sim_promises_get_if; eauto. i. admit. }
+    }
+    { i. hexploit (CLOSEDFUTURE.(closed_future_cur).(closed_future_pln) loc).
+      { eapply NNPP. ii. hexploit ATFLAG; eauto. }
+      i. rewrite H in GET2. rewrite GET2 in GET0. inv GET0. auto.
+    }
+  }
+  intros [vs_tgt1 MAXTGT1]. exists vs_src1, vs_tgt1. splits.
+  { econs.
+    { auto. }
+    { eauto. }
+    { econs; ss.
+      { eapply sim_tview_mon_latest; eauto. }
+      { econs; ss.
+        { i. admit. }
+        { admit. }
+      }
+      { eapply wf_release_vers_versions_le; eauto. }
+    }
+    { eauto. }
+    { ii. eapply MAXTGT1. }
+    { i. hexploit (MAXTGT1 loc); eauto. i. des. auto. }
+    { auto. }
+    { auto. }
+    { auto. }
+  }
+  { i. hexploit VALSRC; eauto. }
+  { i. hexploit (MAXTGT1 loc); eauto. i. des. eapply VALTGT; auto. }
 Admitted.
-(*   hexploit (@max_values_src_exists mem_src1 lc_src0). *)
-(*   intros [vs_src1 MAXSRC1]. des. *)
-(*   assert (VALSRC: forall loc val (VAL: vs_src1 loc = Some val), vs_src0 loc = Some val). *)
-(*   { admit. } *)
-(*   set (vs_tgt1 := fun loc => match vs_src1 loc with *)
-(*                              | Some _ => vs_tgt0 loc *)
-(*                              | None => None *)
-(*                              end). *)
-(*   right. esplits. *)
-(*   { inv SIM. econs. *)
-(*     { eapply sim_timemap_mon_locs; eauto. i. ss. } *)
-(*     { eauto. } *)
-(*     { inv LOCAL. econs; eauto. *)
-(*       { eapply sim_tview_mon_latest; eauto. } *)
-(*       { admit. } *)
-(*       { eapply wf_release_vers_versions_le; eauto. } *)
-(*     } *)
-(*     { eauto. } *)
-(*     { instantiate (1:=vs_tgt1). admit. *)
-(*     } *)
-(*     { i. unfold vs_tgt1. des_ifs. *)
-(*       hexploit VALSRC; eauto. i. hexploit (PERM loc). *)
-(*       rewrite H. auto. *)
-(*     } *)
-(*     { eauto. } *)
-(*     { eauto. } *)
-(*     { eauto. } *)
-(*   } *)
-(*   { admit. } *)
-(* Admitted. *)
